src/Core.Ltt.fst
@@ -2,177 +2,327 @@ module Core.Ltt
 
 open FStar.OrdSet
 open FStar.String
-open FStar.Tactics
+module T = FStar.Tactics
 
-module N = Core.Name
+open Core.Fc
+open Core.Name
 
-(** `ltt` is the core logic that type-checking occurs within.
+(** A predicate that guarentees that a natural number is
+    within bounds for a list. *)
+val valid_index_in : nat -> list 'a -> Tot Type0
+let valid_index_in idx l = idx < List.length l
 
-    `binder` is a binder in the core logic.
+(** Verified way to to get the element at an index that's guarenteed to
+    be within bounds. *)
+private val element_at : l:list 'a -> idx:nat{idx `valid_index_in` l} -> Tot 'a
+let rec element_at l idx =
+  match l, idx with
+  | x :: xs, 0 -> x
+  | x :: xs, _ -> element_at xs (idx-1)
 
-    NOTE: the docs for both of these types are together like
-    this because putting the binder docs where
-    [this wiki page](https://github.com/FStarLang/FStar/wiki/Generating-documentation-with-fsdoc-comments)
-    says to results in the F* subprocess for interactive
-    typechecking exiting.
+private val name_of : l:list local_name -> idx:nat{idx `valid_index_in` l} -> Tot local_name
+let rec name_of l idx = element_at l idx
 
-    TODO: ask about how to fix that. *)
-type ltt =
-  | Var : var:N.name -> ltt
-  | Universe : ltt
-  | Abs : bnd:binder -> var:N.name -> body:ltt -> ltt
-  | App : l:ltt -> r:ltt -> ltt
-and binder =
-  | Pi : ltt -> binder
-  | Lam : binder
+val is_bound_var : local_name -> nat -> list local_name -> Tot Type0
+let is_bound_var n idx ns = idx `valid_index_in` ns /\ n = name_of ns idx
 
-(** Calculate the free variables in an `ltt` term. *)
-val free_variables : t:ltt -> Tot N.name_set
-(** Calculate the free variables in a `ltt` binder. *)
-val binder_free_variables : binder -> Tot N.name_set
-let rec free_variables t =
-  match t with
-  | Var v -> singleton v
-  | Universe -> empty
-  | Abs bnd var body ->
-    let binder_fv = binder_free_variables bnd in
-    union binder_fv (remove var (free_variables body))
-  | App l r -> union (free_variables l) (free_variables r)
-and binder_free_variables b =
-  match b with
-  | Pi ty -> free_variables ty
-  | Lam -> empty
+type var_index (n:local_name) (vars:list local_name) =
+  idx:nat{is_bound_var n idx vars}
 
-(**
-Predicate for checking if a name is free in a `ltt` term.
-*)
-val free_in : N.name -> ltt -> Tot bool
-let free_in v e = mem v (free_variables e)
+type bound_var (vars:list local_name) =
+  | BoundVar : #bound_name:local_name
+             -> index:var_index bound_name vars
+             -> bound_var vars
 
-(**
-Predicate for checking if a `ltt` term is closed--i.e.
-the set of free variables is empty.
-*)
-val is_closed : ltt -> Tot bool
-let is_closed t = free_variables t = empty
+(** Binders are parameterized by the term representation to
+    make them easier to re-use for other representations. *)
+type binder (exp:Type) =
+  | Lam : ty:exp -> binder exp
+  | Let : value:exp -> ty:exp -> binder exp
+  | Pi : ty:exp -> binder exp
 
-(**
-Calculate a name that does not occur within the set of
-names `s` by incrementing the `index` of `n` until it
-is not within `s`.
+(** Map over the expressions in a binder. *)
+val map_binder : ('a -> Tot 'b) -> binder 'a -> Tot (binder 'b)
+let map_binder f = function
+  | Lam ty -> Lam (f ty)
+  | Let v ty -> Let (f v) (f ty)
+  | Pi ty -> Pi (f ty)
 
-This is probably more inefficient than it needs to be,
-because if `n` is in `s`, `find_non_capturing_name`
-removes `n` from `s` before recursing. This is done
-to show termination, but it's a quick hack that I
-should go back and fix if this project ever gets anywhere.
-*)
-val find_non_capturing_name : n:N.name -> s:N.name_set -> Tot N.name (decreases (size s))
-let rec find_non_capturing_name n s =
-  if mem n s
-    then let s': N.name_set = remove n s in
-         find_non_capturing_name (N.inc_name n) s'
-    else n
+(** The core representation that is used for type checking. *)
+type term (vars:list local_name) =
+  | Local : fc -> bound_var vars -> term vars
+  | Ref : fc -> global_name -> term vars
+  | Universe : fc -> term vars
+  | Abs : fc -> var:local_name
+             -> bnd:binder (term vars)
+             -> body:term (var :: vars)
+             -> term vars
+  | App : fc -> l:term vars
+             -> r:term vars
+             -> term vars
+
+type closed_term = term []
 
 (** Size metric for `ltt` terms. *)
-val ltt_size : ltt -> Tot nat
+val term_size : #vars:list local_name -> t:term vars -> Tot nat (decreases t)
 
 (** Size metric for `binder`s. *)
-val binder_size : binder -> Tot nat
+val binder_size : #vars:list local_name
+                -> b:binder (term vars)
+                -> Tot nat (decreases b)
 
-let rec ltt_size = function
-  | Var _ | Universe -> 1
-  | Abs bnd _ body ->
+let rec term_size #vars = function
+  | Local _ _ | Ref _ _ | Universe _ -> 1
+  | Abs _ _ bnd body ->
     let bnd_size = binder_size bnd in
-    bnd_size + ltt_size body + 1
-  | App l r -> ltt_size l + ltt_size r + 1
-and binder_size = function
-  | Pi ty -> 1 + ltt_size ty
-  | Lam -> 1
+    bnd_size + term_size body + 1
+  | App _ l r -> term_size l + term_size r + 1
+and binder_size #vars = function
+  | Pi ty -> 1 + term_size ty
+  | Lam ty -> 1 + term_size ty
+  | Let value ty -> 1 + term_size value + term_size ty
 
-(**
-Replaces all occurances of `replacee` with `substitute`.
-
-This is essentially a specialized version of `subst`;
-I created it bec
-*)
-private val replace_var : N.name -> N.name -> t:ltt -> Tot (ret:ltt{ltt_size ret = ltt_size t})
-let rec replace_var substitute replacee t =
-  let rep = replace_var substitute replacee in
-  match t with
-  | Var v -> if v = replacee then Var substitute else t
-  | Universe -> t
-  | Abs bnd v body ->
-    let bnd' = match bnd with
-      | Pi ty -> Pi (rep ty)
-      | Lam -> Lam in
-    Abs bnd' v (rep body)
-  | App l r -> App (rep l) (rep r)
-
-// This seems to be necessary for the `smt` solver to
-// have enough fuel to verify `subst`.
-#reset-options
-
-(**
-Perform capture-avoiding substitution of `arg` for `v` in  `bod`.
-*)
-val subst : arg:ltt -> v:N.name -> bod:ltt
-  -> Tot ltt (decreases %[ltt_size arg; ltt_size bod])
-
-(**
-Perform capture-avoiding substitution of `arg` for `v` in  `bnd`.
-*)
-val binder_subst : arg:ltt -> v:N.name -> bnd:binder
-  -> Tot binder (decreases %[ltt_size arg; binder_size bnd])
-
-let rec subst arg v t =
-  match t with
-  | Var v' -> if v' = v then arg else t
-  | Universe -> Universe
-  | App l r -> App (subst arg v l) (subst arg v r)
-  | Abs bnd bv body ->
-    if bv = v
-      then t
-      else
-        let bnd' = binder_subst arg v bnd in
-        let fvs = union (free_variables arg) (free_variables body) in
-        let bv' = find_non_capturing_name bv fvs in
-        let body' = replace_var bv' bv body in
-        assert (ltt_size body << ltt_size t);
-        assert (ltt_size body = ltt_size body');
-        assert (ltt_size body' << ltt_size t);
-        Abs bnd' bv' (subst arg v body')
-and binder_subst arg v b =
-  match b with
-  | Pi ty -> Pi (subst arg v ty)
-  | Lam -> Lam
-
-(** Check if two `ltt` terms are alpha equivalent. *)
-val alpha_eq : ltt -> ltt -> Tot bool
-
-(** Check if two `binder`s are alpha equivalent. *)
-val binder_alpha_eq : binder -> binder -> Tot bool
-
-let rec alpha_eq t1 t2 =
-  match t1, t2 with
-  | Abs b1 v1 e1, Abs b2 v2 e2 ->
-    binder_alpha_eq b1 b2
-    && alpha_eq e1 (subst (Var v1) v2 e2)
-  | App l1 r1, App l2 r2 -> alpha_eq l1 l2 && alpha_eq r1 r2
-  | _ -> t1 = t2
-and binder_alpha_eq b1 b2 =
-  match b1, b2 with
-  | Pi ty1, Pi ty2 -> alpha_eq ty1 ty2
-  | Lam, Lam -> true
+(** Alpha equality implementation for terms. *)
+val alpha_eq : #vs1:list local_name -> #vs2:list local_name
+             -> t1:term vs1 -> t2:term vs2
+             -> Tot bool (decreases (term_size t1 + term_size t2))
+let rec alpha_eq #vs1 #vs2 t t' =
+  match t, t' with
+  | Local _ bv1, Local _ bv2 -> bv1.index = bv2.index
+  | Ref _ tln1, Ref _ tln2 -> tln1 = tln2
+  | Abs _ _ bnd1 body1, Abs _ _ bnd2 body2 ->
+    alpha_eq body1 body2 &&
+    (match bnd1, bnd2 with
+    | Lam t1, Lam t2 -> alpha_eq t1 t2
+    | Let v1 t1, Let v2 t2 -> alpha_eq v1 v2 && alpha_eq t1 t2
+    | Pi t1, Pi t2 -> alpha_eq t1 t2
+    | _ -> false)
+  | App _ l1 r1, App _ l2 r2 ->
+    alpha_eq l1 l2 && alpha_eq r1 r2
   | _ -> false
 
-(** Assorted assertions. *)
-[@"opaque_to_smt"]
-let _ =
-  let x = N.intro "x" in
-  let y = N.intro "y" in
-  let id = Abs Lam x (Var x) in
-  let xy = Abs Lam x (Var y) in
-  assert (subst (Universe) y xy = Abs Lam x (Universe));
-  assert (subst (Universe) x id = id)
-  
+(** Insert a variable into the local context and adjust
+    the bound variable `var` to still be accurate in the
+    new environment. *)
+val insert_var : #outer:list local_name
+               -> #inner:list local_name
+               -> #existing_name:local_name
+               -> new_name:local_name
+               -> idx:var_index existing_name (outer @ inner)
+               -> Tot (var_index existing_name (outer @ new_name :: inner))
+let rec insert_var #outer #inner #existing_name new_name idx =
+  match outer, idx with
+  // If `outer` is empty, that means that we simply need to bump
+  // `idx` by one to account for the new name that has been added
+  // to the scope.
+  | [], i -> i+1
+  // If `existing_name` (the one we're adjusting the index of) is
+  // at the top of the `outer` scope, then we just leave it's index
+  // as-is.
+  | x :: xs, 0 -> assert (x = existing_name); 0
+  // If the variable is further down the scope stack, we remove the
+  // head of `outer` and decrement the index by one, then recurse.
+  // Once we have the result from that, we add one to it.
+  | x :: xs, i ->
+    let i' = insert_var #xs #inner #existing_name new_name (i-1) in
+    i'+1
+
+(** A lemma used in the `weaken_var` function that basically says
+    that all it takes to adjust an index to having added names to
+    the outer scope is to increment the index by the length of
+    the outer scope. *)
+private val weaken_var_lemma : ns:list local_name
+                             -> Lemma
+  (ensures forall inner existing (idx:var_index existing inner).
+    let bump = List.length ns in
+    is_bound_var existing (idx+bump) (ns@inner))
+let rec weaken_var_lemma ns =
+  // We prove the lemma by performing induction over the structure
+  // of `ns`.
+  match ns with
+  // If we're not adding anything to the scope, the index
+  // stays the same--a trivial case.
+  | [] -> ()
+  // For each element we need to add one to the index, which is
+  // trivial for the SMT solver to infer once we tell it to perform
+  // induction.
+  | x :: xs -> weaken_var_lemma xs; ()
+
+(** Add additional names to the outer scope of a variable. *)
+val weaken_var : #inner:list local_name
+               -> #existing_name:local_name
+               -> ns:list local_name
+               -> idx:var_index existing_name inner
+               -> Tot (var_index existing_name (ns @ inner))
+let weaken_var #inner #existing_name ns idx =
+  weaken_var_lemma ns;
+  idx + List.length ns
+
+(** Insert a series of variable names inside of an existing scope.
+
+    Adjusts the passed variable index to still point to the correct
+    point in the scope for the corresponding name. *)
+val insert_var_names : #outer:list local_name
+                     -> #inner:list local_name
+                     -> #existing_name:local_name
+                     -> ns:list local_name
+                     -> idx:var_index existing_name (outer @ inner)
+                     -> Tot (var_index existing_name (outer @ ns @ inner))
+let rec insert_var_names #outer #inner #existing_name ns idx =
+  match outer, idx with
+  | [], _ -> weaken_var ns idx
+  | x :: xs, 0 -> 0
+  | y :: ys, _ ->
+    let idx' = insert_var_names #ys #inner #existing_name ns (idx-1) in
+    idx' + 1
+
+(** Insert multiple names into a term's scope. *)
+private val thin : #outer:list local_name
+                 -> #inner:list local_name
+                 -> ns:list local_name
+                 -> t:term (outer @ inner)
+                 -> Tot (term (outer @ ns @ inner)) (decreases %[term_size t])
+let rec thin #outer #inner ns t =
+  match t with
+  | Local fc bv -> let idx' = insert_var_names ns bv.index in
+                  Local fc (BoundVar idx')
+  | Ref fc gn -> Ref fc gn
+  | Universe fc -> Universe fc
+  | Abs fc var bnd body ->
+    let outer' = var :: outer in
+    let bnd' = match bnd with
+      | Pi ty -> Pi (thin ns ty)
+      | Let v ty -> Let (thin ns v) (thin ns ty)
+      | Lam ty -> Lam (thin ns ty) in
+    let body' = thin #outer' #inner ns body in
+    Abs fc var bnd' body'
+  | App fc l r -> App fc (thin ns l) (thin ns r)
+
+(** Add a single variable to the scope of the term.
+
+    A surprisingly useful utility function. *)
+private val weaken_term : #vars:list local_name
+                        -> ns:list local_name
+                        -> term vars
+                        -> Tot (term (ns @ vars))
+let weaken_term #vars ns t = thin #[] #vars ns t
+
+(** Lemma for renaming variable indices. *)
+private val rename_var_index_lemma : #xs:list local_name
+                                   -> #ys:list local_name
+                                   -> #cur_name:local_name
+                                   -> idx:nat{is_bound_var cur_name idx xs}
+                                   -> Lemma
+  (requires idx `valid_index_in` ys)
+  (ensures is_bound_var (name_of ys idx) idx ys) (decreases %[xs; ys])
+let rec rename_var_index_lemma #xs #ys #cur_name idx =
+  match xs, ys, idx with
+  | x :: xs', _, 0 -> assert (x = cur_name)
+  | x :: xs', y :: ys', _ ->
+    rename_var_index_lemma #xs' #ys' #cur_name (idx - 1)
+
+private type subst_env (vars:list local_name) (drops:list local_name) =
+  terms:list (term vars){List.length terms = List.length drops}
+
+private val sub_index_lemma : #outer:list local_name
+                            -> #inner:list local_name
+                            -> #name:local_name
+                            -> idx:nat
+                            -> Lemma
+  (requires (is_bound_var name idx (outer @ inner))
+            /\ (idx `valid_index_in` outer))
+  (ensures (is_bound_var name idx outer))
+  (decreases %[outer])
+let rec sub_index_lemma #outer #inner #name idx =
+  if idx = 0 then () else
+    let idx':nat = idx - 1 in
+    let outer' = List.Tot.tail outer in
+    sub_index_lemma #outer' #inner #name idx'
+
+private val super_index_lemma : #outer:list local_name
+                              -> #inner:list local_name
+                              -> #name:local_name
+                              -> idx:nat
+                              -> Lemma
+  (requires (is_bound_var name idx outer))
+  (ensures (is_bound_var name idx (outer @ inner)))
+  (decreases outer)
+let rec super_index_lemma #outer #inner #name idx =
+  if idx = 0 then () else
+    let idx':nat = idx - 1 in
+    let outer' = List.Tot.tail outer in
+    super_index_lemma #outer' #inner #name idx'
+
+private val strip_index_lemma : outer:list local_name
+                              -> inner:list local_name
+                              -> name:local_name
+                              -> idx:var_index name (outer @ inner)
+                              -> Lemma
+  (requires idx >= List.length outer)
+  (ensures is_bound_var name (idx - List.length outer) inner)
+  (decreases outer)
+let rec strip_index_lemma outer inner name idx =
+  match outer with
+  | [] -> ()
+  | x :: xs ->
+    let idx' = idx-1 in
+    strip_index_lemma xs inner name idx'
+
+private val try_to_drop : #outer:list local_name
+                        -> #vars:list local_name
+                        -> #drop:list local_name
+                        -> #name:local_name
+                        -> fc -> idx:var_index name (outer @ drop @ vars)
+                        -> subst_env vars drop
+                        -> Tot (term (outer @ vars))
+let try_to_drop #outer #vars #drop #name fc idx env =
+  let start = List.length outer in
+  let stop = List.length outer + List.length drop in
+
+  let all_vars = outer @ drop @ vars in
+  let new_vars = outer @ vars in
+
+  // If `idx` is in `outer`
+  if idx < start then (
+    assert (idx `valid_index_in` outer);
+    sub_index_lemma #outer #(drop @ vars) #name idx;
+    let outer_idx: var_index name outer = idx in
+    super_index_lemma #outer #vars #name outer_idx;
+    let new_idx: var_index name new_vars = outer_idx in
+    (Local fc (BoundVar new_idx)) <: term new_vars
+
+  // If `idx` is in `drop`
+  ) else if idx < stop then (
+    let tm_index = idx - start in
+    let tm = element_at env tm_index in
+    (weaken_term outer tm) <: term new_vars
+
+  // If `idx` is in `vars`
+  ) else (
+    List.Tot.append_assoc outer drop vars;
+    strip_index_lemma (outer @ drop) vars name idx;
+    let vars_index: var_index name vars = idx - stop in
+    weaken_var_lemma outer;
+    let new_idx: var_index name new_vars = vars_index + start in
+    (Local fc (BoundVar new_idx)) <: term new_vars
+  )
+
+private val subst : #outer:list local_name
+                  -> #vars:list local_name
+                  -> #drop:list local_name
+                  -> subst_env vars drop
+                  -> t:term (outer @ drop @ vars)
+                  -> Tot (term (outer @ vars)) (decreases t)
+let rec subst #outer #vars #drop env = function
+  | Local fc (BoundVar idx) -> try_to_drop fc idx env
+  | Ref fc gn -> Ref fc gn
+  | Universe fc -> Universe fc
+  | Abs fc var bnd body ->
+    let outer' = var :: outer in
+    let bnd' = match bnd with
+      | Pi ty -> Pi (subst env ty)
+      | Let v ty -> Let (subst env v) (subst env ty)
+      | Lam ty -> Lam (subst env ty) in
+    let body' = subst #outer' env body in
+    Abs fc var bnd' body'
+  | App fc l r -> App fc (subst env l) (subst env r)
