src/Core.Name.fst
@@ -4,6 +4,7 @@ open FStar.OrdSet
 
 module M = FStar.OrdMap
 module O = FStar.Order
+module T = FStar.Tactics
 
 (** Represents an identifier.
 
@@ -15,89 +16,291 @@ type base_name = {
   str : string;
 }
 
-(** Useful information about a name, such as
-    its origin. *)
-type name_sort =
-  | UserGen
-  | MachineGen
+(** A series of module names that indicates a namespace. *)
+type namespace_path = list string
 
-(** A name used to identify something. *)
-type name = {
-  base : base_name;
-  sort : name_sort
+(** A local (un-qualified) name. *)
+type local_name =
+  | UserGen : base_name -> local_name
+  | MachineGen : base_name -> local_name
+
+(** A global (qualified) name.
+
+    TODO: consider renaming this to `qualified_name`. *)
+type global_name = {
+  namespace : namespace_path;
+  local_name : local_name
 }
+
+(** A global or local name. *)
+type any_name =
+  | LocalName : local_name -> any_name
+  | GlobalName : global_name -> any_name
+
+(** Get the base name of a local_name. *)
+val get_base_name : local_name -> Tot base_name
+let rec get_base_name = function
+  | UserGen bn -> bn
+  | MachineGen bn -> bn
 
 (** Apply a modification to the base name. *)
-val mod_base_name : (base_name -> Tot base_name) -> name -> Tot name
-let mod_base_name f n = { sort = n.sort; base = f n.base }
+val mod_base_name : (base_name -> Tot base_name) -> local_name -> Tot local_name
+let rec mod_base_name f = function
+  | UserGen bn -> UserGen (f bn)
+  | MachineGen bn -> MachineGen (f bn)
 
-(** Introduce a new user-generated name.
+(** Introduce a new user-generated local_name.
 
     Initializes the name with `index` at `0`. *)
-val intro : string -> Tot name
-let intro s = {
-  sort = UserGen;
-  base = {
-    str = s;
-    index = 0
-  }
-}
+val intro : string -> Tot local_name
+let intro s = UserGen ({
+  str = s;
+  index = 0
+})
 
-(** Introduce a new machine-generated name. *)
-val mintro : string -> Tot name
-let mintro s = {
-  sort = MachineGen;
-  base = {
-    str = s;
-    index = 0
-  }
-}
+(** Introduce a new machine-generated local_name. *)
+val mintro : string -> Tot local_name
+let mintro s = MachineGen ({
+  str = s;
+  index = 0
+})
 
-(** Increment the index of a name. *)
-val inc_name : name -> Tot name
+(** Increment the index of a local_name. *)
+val inc_name : local_name -> Tot local_name
 let inc_name = mod_base_name
-  (fun n -> { index = n.index+1; str = n.str })
+  (fun n -> { n with index = n.index+1 })
 
-(** A total ordering on names. *)
-abstract val name_order : name -> name -> Tot bool
-let name_order n1 n2 =
-  let compare_sort s1 s2 =
-    let rank (s:name_sort): nat =
-      match s with
-      | UserGen -> 1
-      | MachineGen -> 0 in
+private type ordering (a:eqtype) = a -> a -> Tot O.order
 
-    O.compare_int (rank s1) (rank s2) in
+unfold private let ordering_anti_symmetry (#a:eqtype) (f:ordering a) (x:a) (y:a) =
+  f x y = O.Eq ==> x = y
 
-  let compare_string s1 s2 =
-    Order.order_from_int (String.compare s1 s2) in
+unfold private let ordering_transitivity (#a:eqtype) (f:ordering a) (x:a) (y:a) (z:a): GTot Type0 =
+  match f x y, f y z with
+  | O.Eq, o -> f x z = o
+  | o, O.Eq -> f x z = o
+  | o1, o2 -> if o1 = o2 then f x z = o1 else True
 
-  let compare_name n1 n2 =
-    O.lex (compare_sort n1.sort n2.sort)
-      (fun () -> O.lex (O.compare_int n1.base.index n2.base.index)
-        (fun () -> compare_string n1.base.str n2.base.str)) in
+unfold private let ordering_totality (#a:eqtype) (f:ordering a) (x:a) (y:a): GTot Type0 =
+  match f x y, f y x with
+  | O.Eq, O.Eq
+  | O.Gt, O.Lt
+  | O.Lt, O.Gt -> True
+  | _ -> False
 
-  O.gt (compare_name n1 n2)
+private type total_ordering_prop (a:eqtype) (f:ordering a) =
+  (forall x y. ordering_anti_symmetry f x y) // anti-symmetry
+  /\ (forall x y z. ordering_transitivity f x y z) // transitivity
+  /\ (forall x y. ordering_totality f x y) // totality
 
-(*
-I can't figure out how to prove that string
-comparison is total, so I'm just making this
-an axiom.
+private val total_order_form : #a:eqtype -> (ordering a) -> Tot (a -> a -> Tot bool)
+let total_order_form #a f x y = O.ge (f x y)
 
-NOTE: if this is an `fsdoc` comment, it again
-seems to crash the F* subprocess for interactive
-typechecking.
+private val ordering_is_total : a:eqtype -> (ordering a) -> GTot Type0
+let ordering_is_total a f = total_ordering_prop a f
+                            /\ total_order a (total_order_form f)
 
-TODO: figure out how to fix that.
-*)
-assume NameOrderIsTotal: total_order name name_order
+private let order_transitivity (a:eqtype) (g:(a -> a -> Tot bool)) (x:a) (y:a) (z:a) =
+  g x y /\ g y z ==> g x z
 
-let name_order_cmp: cmp name = name_order
+private val order_transitivity_lemma : #a:eqtype -> g:(a -> a -> Tot bool)
+                                     -> Lemma
+  (requires forall x y z. order_transitivity a g x y z)
+  (ensures forall x y z. g x y /\ g y z ==> g x z)
+let order_transitivity_lemma #a g =
+  assert_norm ((forall x y z. order_transitivity a g x y z)
+         ==> (forall x y z. g x y /\ g y z ==> g x z));
+  ()
 
-(** A type alias for a set of names.
+private val ordering_transitivity_lemma : #a:eqtype -> f:ordering a
+                                        -> x:a -> y:a -> z:a
+                                        -> Lemma
+  (requires ordering_transitivity f x y z)
+  (ensures (let g = total_order_form f in g x y /\ g y z ==> g x z))
+  [SMTPat (order_transitivity a (total_order_form f) x y z)]
+let ordering_transitivity_lemma #a f x y z = ()
+
+private val total_order_derivation_lemma : #a:eqtype -> f:ordering a -> Lemma
+  (requires total_ordering_prop a f)
+  (ensures total_order a (total_order_form f))
+  [SMTPat (total_ordering_prop a f)]
+let total_order_derivation_lemma #a f =
+  let g = total_order_form f in
+  // Prove that anti-symmetry converts
+  assert (forall x y. ordering_anti_symmetry f x y ==> (g x y /\ g y x ==> x = y));
+  assert (forall x y. g x y /\ g y x ==> x = y);
+
+  // Prove that transitivity converts
+  assert (forall x y z. ordering_transitivity f x y z ==> (g x y /\ g y z ==> g x z));
+  assert (forall x y z. order_transitivity a g x y z);
+  order_transitivity_lemma g;
+  assert (forall x y z. g x y /\ g y z ==> g x z);
+
+  // Prove that totality converts
+  assert (forall x y. ordering_totality f x y ==> (g x y \/ g y x));
+  assert (forall x y. g x y \/ g y x);
+
+  ()
+
+private type total_ordering (a:eqtype) =
+  f:(a -> a -> Tot O.order){ordering_is_total a f}
+
+private val compare_string : total_ordering string
+let compare_string = admit ();
+  fun s1 s2 -> O.order_from_int (String.compare s1 s2)
+
+private val compare_nat_total_lemma : unit -> Lemma
+  (ensures total_ordering_prop nat O.compare_int)
+let compare_nat_total_lemma () = ()
+
+private val compare_base_name : total_ordering base_name
+let compare_base_name b1 b2 =
+  match O.compare_int b1.index b2.index with
+  | O.Lt -> O.Lt
+  | O.Gt -> O.Gt
+  | O.Eq -> compare_string b1.str b2.str
+
+private val compare_local_name' : ordering local_name
+let compare_local_name' n1 n2 =
+  let rank (n:local_name): nat =
+    match n with
+    | UserGen _ -> 1
+    | MachineGen _ -> 0 in
+
+    match n1, n2 with
+    | UserGen b1, UserGen b2 -> compare_base_name b1 b2
+    | MachineGen b1, MachineGen b2 -> compare_base_name b1 b2
+    | _ -> O.compare_int (rank n1) (rank n2)
+
+private val compare_local_name_total_lemma : unit -> Lemma
+  (ensures ordering_is_total local_name compare_local_name')
+let compare_local_name_total_lemma () = ()
+
+private val compare_local_name : total_ordering local_name
+let compare_local_name =
+  compare_local_name_total_lemma ();
+  compare_local_name'
+
+private val compare_list_anti_symmetry_lemma : #a:eqtype -> g:total_ordering a
+                                     -> l1:list a -> l2:list a
+                                     -> Lemma
+  (ensures (let f = O.compare_list g in
+           (ordering_anti_symmetry f l1 l2)))
+let rec compare_list_anti_symmetry_lemma #a g l1 l2 =
+  let f = O.compare_list g in
+  match l1, l2 with
+  | [], [] -> ()
+  | [], _ -> ()
+  | _, [] -> ()
+  | x :: xs, y :: ys -> compare_list_anti_symmetry_lemma g xs ys; ()
+
+private val compare_list_totality_lemma : #a:eqtype -> g:total_ordering a
+                                     -> l1:list a -> l2:list a
+                                     -> Lemma
+  (ensures (let f = O.compare_list g in
+           (ordering_totality f l1 l2)))
+let rec compare_list_totality_lemma #a g l1 l2 =
+  let f = O.compare_list g in
+  match l1, l2 with
+  | [], [] -> ()
+  | [], _ -> ()
+  | _, [] -> ()
+  | x :: xs, y :: ys -> compare_list_totality_lemma g xs ys; ()
+
+private val compare_list_transitivity_lemma : #a:eqtype -> g:total_ordering a
+                                            -> l1:list a -> l2:list a -> l3:list a
+                                            -> Lemma
+  (ensures (let f = O.compare_list g in
+           ordering_transitivity f l1 l2 l3))
+let rec compare_list_transitivity_lemma #a g l1 l2 l3 =
+  let f = O.compare_list g in
+  match l1, l2, l3 with
+  | x::xs, y::ys, z::zs ->
+    compare_list_transitivity_lemma g xs ys zs;
+    (match g x y, g y z with
+    | O.Eq, o -> assert (g x z = o); ()
+    | o, O.Eq -> assert (g x z = o); ()
+    | o1, o2 -> if o1=o2
+      then (assert (g x z = o1); ())
+      else ())
+  | _ -> ()
+
+private val compare_list_total_lemma : #a:eqtype -> g:total_ordering a
+                                     -> Lemma
+  (ensures ordering_is_total (list a) (O.compare_list g))
+let compare_list_total_lemma #a g =
+  let f = O.compare_list g in
+  assert (forall x y. ordering_anti_symmetry (O.compare_list g) x y)
+    by (let _ = T.forall_intros () in
+       T.apply_lemma (`compare_list_anti_symmetry_lemma));
+  assert (forall x y. ordering_totality f x y)
+    by (let _ = T.forall_intros () in
+       T.apply_lemma (`compare_list_totality_lemma));
+  assert (forall x y z. ordering_transitivity f x y z)
+    by (ignore (T.forall_intros ());
+       T.apply_lemma (`compare_list_transitivity_lemma));
+  assert (total_ordering_prop (list a) f);
+  ()
+
+private val compare_global_name' : ordering global_name
+let compare_global_name' gn1 gn2 =
+  match compare_local_name gn1.local_name gn2.local_name with
+  | O.Lt -> O.Lt
+  | O.Gt -> O.Gt
+  | O.Eq ->
+    O.compare_list compare_string gn1.namespace gn2.namespace
+
+private val compare_global_name_lemma : unit -> Lemma
+  (ensures ordering_is_total global_name compare_global_name')
+let compare_global_name_lemma () = compare_list_total_lemma compare_string
+
+private val compare_global_name : total_ordering global_name
+let compare_global_name =
+  compare_global_name_lemma ();
+  compare_global_name'
+
+private val compare_any_name : total_ordering any_name
+let compare_any_name an1 an2 =
+  match an1, an2 with
+  | GlobalName gn1, GlobalName gn2 -> compare_global_name gn1 gn2
+  | GlobalName _, LocalName _ -> O.Gt
+  | LocalName _, GlobalName _ -> O.Lt
+  | LocalName ln1, LocalName ln2 -> compare_local_name ln1 ln2
+
+private unfold let order_map (#t:eqtype) (ordering:total_ordering t) (a:Type) =
+  M.ordmap t a (total_order_form ordering)
+
+(** A total ordering on local names.
+
+    Needs to be `abstract` or it causes problems with
+    monads. *)
+abstract val local_name_order : cmp local_name
+let local_name_order = total_order_form compare_local_name
+
+(** A total ordering on global names.
+
+    Needs to be `abstract` or it causes problems with
+    monads. *)
+abstract val global_name_order : cmp global_name
+let global_name_order = total_order_form compare_global_name
+
+(* A total ordering on `any_name`s.
+
+    Needs to be `abstract` or it causes problems with
+    monads.
+abstract val any_name_order : cmp any_name
+let any_name_order = total_order_form compare_any_name *)
+
+(** A type alias for a set of local names.
 
     Generally used when calculating free variables. *)
-let name_set: Type0 = ordset name name_order
+let local_name_set: Type0 = ordset local_name local_name_order
 
-(** A type alias for a map from names to `a`. *)
-type name_map (a:Type) = M.ordmap name a name_order
+(** A type alias for a map from local names to `a`. *)
+type local_name_map (a:Type) = M.ordmap local_name a local_name_order
+
+(** A type alias for a map from global names to `a`. *)
+type global_name_map (a:Type) = M.ordmap global_name a global_name_order
+
+(** A type alias for a map from global and local names to 'a'. *)
+type any_name_map = order_map compare_any_name
