src/Core.Context.fst
@@ -1,0 +1,54 @@
+module Core.Context
+
+open Core.Fc
+open Core.Name
+open Core.Ltt
+
+(** The actual "implementation" of top-level definitions
+    (i.e. whether it's a function, or a data constructor).
+
+    Future cases are things like type constructors and
+    data constructors. *)
+type def =
+  | Function : body:closed_term -> def
+
+(** Contains extra context *)
+type global_def = {
+  location : fc;
+  qualified_name : global_name;
+  type': closed_term;
+  definition: def;
+}
+
+(** Create a global definition with no location and with
+    `["Main"]` for the namespace. *)
+val mk_gdef : string -> closed_term -> def -> Tot global_def
+let mk_gdef name ty d = {
+  location = EmptyFc;
+  qualified_name = {
+    namespace = ["Main"];
+    local_name = intro name;
+  };
+  type' = ty;
+  definition = d;
+}
+
+val term_for_gdef : global_def -> Tot closed_term
+let term_for_gdef gdef =
+  match gdef.definition with
+  | Function body -> body
+
+unopteq type context = {
+  content: any_name_map global_def;
+}
+
+(** Initialize a context based on a list of names and definitions. *)
+val init_context : list (any_name * global_def)
+                 -> context
+let init_context l =
+  let f c (n, d) = OrdMap.update n d c in
+  let content = List.Tot.fold_left f OrdMap.empty l in
+  { content = content }
+
+val lookup_gdef : any_name -> context -> Tot (option global_def)
+let lookup_gdef name ctxt = OrdMap.select name ctxt.content
