src/Core.Fc.fst
@@ -1,0 +1,9 @@
+module Core.Fc
+
+type file_pos = { row:nat; col:nat }
+
+type file_name = string
+
+type fc =
+  | MkFc : file:file_name -> start:file_pos -> stop:file_pos -> fc
+  | EmptyFc : fc
