src/Core.Raw.fst
@@ -1,0 +1,18 @@
+module Core.Raw
+
+open Core.Fc
+open Core.Name
+open Core.Ltt
+
+type raw_term (vars:list local_name) =
+  | RVar : fc -> any_name -> raw_term vars
+  | RUniverse : fc -> raw_term vars
+  | RAbs : fc -> var:local_name
+              -> bnd:binder (raw_term vars)
+              -> body:raw_term (var :: vars)
+              -> raw_term vars
+  | RApp : fc -> l:raw_term vars
+              -> r:raw_term vars
+              -> raw_term vars
+
+type closed_raw_term = raw_term []
