src/Core.TypeCheck.fst
@@ -1,0 +1,32 @@
+module Core.TypeCheck
+
+open Core.Fc
+open Core.Name
+open Core.Raw
+open Core.Ltt
+open Core.Tc
+open Core.Environment
+
+(** A mapping of the in-scope names to the type that they
+    are bound to. *)
+private type local_ctxt vars = local_env raw_term vars
+
+//private val expand_binder : #vars:list local_name -> #
+
+private val lookup_ty : #vars:list local_name
+                      -> fc
+                      -> any_name
+                      -> local_ctxt vars
+                      -> TcNull (raw_term vars)
+let lookup_ty #vars fc n ctx =
+  let res = match n with
+  | LocalName ln ->
+    (match env_lookup ln ctx with
+    Some v -> v
+    None -> None)
+  | _ -> None in
+  match res with
+  | Some v -> v
+  | None -> lookup' fc n
+
+val infer_type : body:raw_term -> env:local_scope -> TcNull (ty:raw_term)
